compose/SimSystem.v
@@ -7,7 +7,7 @@ Require Import Smallstep Simulation.
 Require Import CoqlibC.
 
 Require Import Mod ModSem Skeleton System.
-Require Import SimMem Sound SimSymb.
+Require Import SimMem Sound SimSymb Syntax.
 
 Set Implicit Arguments.
 
@@ -16,4 +16,17 @@ Section SIM.
   Context `{SM: SimMem.class}.
   Context `{SU: Sound.class}.
   Context {SS: SimSymb.class SM}.
+
+  Variables p: program.
+  System.module p
+  Definition mp: ModPair.t := SimSymb.mk_mp (RTLC.module prog) (RTLC.module tprog).
+
+  Theorem sim_mod: ModPair.sim mp.
+  Proof.
+    econs; ss.
+    - r. eapply Sk.match_program_eq; eauto. ii. destruct f1; ss.
+      + clarify. right. esplits; eauto.
+      + clarify. left. esplits; eauto.
+    - ii. inv SIMSKENVLINK. eapply sim_modsem; eauto.
+  Qed.
 End SIM.
