proof/SimSymb.v
@@ -100,11 +100,12 @@ Module SimSymb.
           (SIMSKENV: sim_skenv sm ss skenv_src skenv_tgt),
           <<DEF: skenv_func_bisim sm.(SimMem.sim_val) skenv_src skenv_tgt>>;
 
-      system_sim_skenv: forall sm ss sk_src skenv_src sk_tgt skenv_tgt
-          (LOADSRC: (Sk.load_skenv sk_src) = skenv_src)
-          (LOADTGT: (Sk.load_skenv sk_tgt) = skenv_tgt)
+      system_sim_skenv: forall sm ss skenv_src skenv_tgt
+          (SIMSK: wf ss)
+          (LOADSRC: (Sk.load_skenv ss.(src)) = skenv_src)
+          (LOADTGT: (Sk.load_skenv ss.(tgt)) = skenv_tgt)
           (SIMSKENV: sim_skenv sm ss skenv_src skenv_tgt),
-          <<SIMSKENV: sim_skenv sm ss (System.skenv sk_src skenv_src) (System.skenv sk_tgt skenv_tgt)>>;
+          exists ss_sys, <<SIMSKENV: sim_skenv sm ss_sys (System.skenv ss.(src) skenv_src) (System.skenv ss.(tgt) skenv_tgt)>>;
       system_axiom: forall
           sm0 ss_sys skenv_sys_src skenv_sys_tgt
           args_src args_tgt tr retv_src ef
